\addchap[Appendix A:$\quad$Answers and Hints to Selected Exercises]{Appendix A}
\textsf{\textbf{\Large Answers and Hints to Selected Exercises}}
\begin{multicols}{2}
\section*{Chapter \ref{chapter:vectors}}
\subsection*{Section \ref{sec1dot1} (p. \pageref{sec1dot1})}
\textbf{1.} 
(a)~$\sqrt{5}$; \quad 
(b)~$\sqrt{5}$; \quad 
(c)~$\sqrt{17}$; \quad 
(d)~$1$;\quad
(e)~$2 \sqrt{17}$; \quad 
\textbf{2.}~Yes; \quad 
\textbf{3.}~No.
\subsection*{Section \ref{sec1dot2} (p. \pageref{sec1dot2})}
\textbf{1.} 
(a)~$(-4,4,-3)$; \quad 
(b)~$(2,6,-1)$;\quad
(c)~$\left ( \frac{-1}{\sqrt{30}},\frac{5}{\sqrt{30}},
\frac{-2}{\sqrt{30}}\right )$; \quad 
(d)~$\frac{\sqrt{41}}{2}$; \quad 
(e)~$\frac{\sqrt{41}}{2}$;\quad
(f)~$(14,-6,8)$; \quad
(g)~$(-7,3,-4)$; \quad
(h)~$(-1,-6,1)$; \quad 
(i)~$(-2,-4,2)$; \quad 
(j)~No.\quad
\textbf{3.} No. $\norm{\textbf{v}} +
\norm{\textbf{w}}$ is larger.

\subsection*{Section \ref{sec1dot3} (p. \pageref{sec1dot3})}
\textbf{1.}~$10$; \quad 
\textbf{3.}~$73.4\Degrees$; \quad 
\textbf{5.}~$90\Degrees$; \quad 
\textbf{7.}~$0\Degrees$;\quad
\textbf{9.}~Yes, since $\Dotprod{\textbf{v}}{\textbf{w}} = 0$;\quad
\textbf{11.}~$\abs{\Dotprod{\textbf{v}}{\textbf{w}}} =
0 < \sqrt{21}\sqrt{5} = \norm{\textbf{v}}\,\norm{\textbf{w}}$;\quad
\textbf{13.}~$\norm{\textbf{v} + \textbf{w}} = \sqrt{26}
< \sqrt{21} + \sqrt{5} = \norm{\textbf{v}} + \norm{\textbf{w}}$;
\textbf{15.}~Hint: use DefinitionЁ\ref{defn:dotprod};\quad
\textbf{24.}~Hint: See Theorem \ref{thm:dotnorm}(c).

\subsection*{Section \ref{sec1dot4} (p. \pageref{sec1dot4})}
\textbf{1.}~$(-5,-23,-24)$; \quad 
\textbf{3.}~$(8,4,-5)$; \quad 
\textbf{5.}~$\textbf{0}$;\quad
\textbf{7.}~$16.72$; \quad
\textbf{9.}~$4\sqrt{5}$; \quad 
\textbf{11.}~$9$; \quad 
\textbf{13.}~$0$ and $(8,-10,2)$;\quad 
\textbf{15.}~$14$;\quad
\textbf{31.}~A circle of radius $\tfrac1{\norm{\mathbf{v}}}$ centered at the origin in the normal plane to $\mathbf{v}$. 

\subsection*{Section \ref{sec1dot5} (p. \pageref{sec1dot5})}
\textbf{1.}
(a)~$(2,3,-2) + t(5,4,-3)$; \quad 
(b)~$x = 2 + 5t,$ $y = 3 + 4t$, $z = -2 - 3t$; \quad 
(c)~$\frac{x - 2}{5} = \frac{y - 3}{4} = \frac{z + 2}{-3}$;\quad
\textbf{3.} 
(a)~$(2,1,3) + t(1,0,1)$; \quad 
(b)~$x = 2 + t,$ $y = 1, \, z = 3 + t$;\quad 
(c)~$x - 2 = z - 3, \, y = 1$;\quad
\textbf{5.}~$x = 1 + 2t, \, y = -2 + 7t, \, z = -3 + 8t$;\quad
\textbf{7.}~7.65; \quad
\textbf{9.}~$(1,2,3)$;\quad
\textbf{11.}~$4x - 4y + 3z - 10 = 0$;\quad
\textbf{13.}~$x - 2y - z + 2 = 0$;\quad
\textbf{15.}~$11x - 24y + 21z - 26 = 0$; \quad 
\textbf{17.}~$9/\sqrt{35}$;\quad
\textbf{19.}~$x = 5t$, $y = 2 + 3t$, $z = -7t$;\quad
\textbf{21.}~$(10,-2,1)$.

\subsection*{Section \ref{sec1dot6} (p. \pageref{sec1dot6})}
\textbf{1.}~radius: $1$, center: $(2,3,5)$; \quad \textbf{3.}~radius: $5$, center: $(-1,-1,-1)$; \quad \textbf{5.}~No intersection;\quad
\textbf{7.}~circle $x^2 + y^2 = 4$ in the planes $z = \pm \sqrt{5}$; \quad
\textbf{9.}~lines
$\frac{x}{a} = \frac{y}{b}$, $z = 0$ and $\frac{x}{a} = -\frac{y}{b}$, $z = 0$; \quad
\textbf{13.}$\left( \frac{2a}{2 - c}, \frac{2b}{2 - c}, 0 \right)$.

\subsection*{Section \ref{sec1dot7} (p. \pageref{sec1dot7})}
\textbf{1.} 
(a)~$(4,\frac{\pi}{3},-1)$; \quad 
(b)~$(\sqrt{17},\frac{\pi}{3},1.816)$; \quad
\textbf{3.}
(a)~$(2\sqrt{7},\frac{11\pi}{6},0)$; \quad 
(b)~$(2\sqrt{7},\frac{11\pi}{6},\frac{\pi}{2})$; \quad
\textbf{5.} 
(a)~$r^2 + z^2 = 25$; \quad
(b)~$\rho = 5$; \quad
\textbf{7.} 
(a)~$r^2 + 9z^2 = 36$; \quad 
(b)~$\rho^2 ( 1 + 8 \cos^2 \phi ) = 36$; \quad
\textbf{10.}~$(a,\theta,a \cot \phi )$;\quad 
\textbf{12.}~Hint: Use the distance formula for Cartesian coordinates.

\section*{Chapter \ref{chapter:curves}}
\subsection*{Section \ref{sec1dot8} (p. \pageref{sec1dot8})}
\textbf{1.}~$\textbf{f}\,'(t) = (1,2t,3t^2)$, $x = 1 + t$, $y = z = 1$; \quad
\textbf{3.}~$\textbf{f}\,'(t) =
(-2\sin 2t,2\cos 2t,1)$; $x = 1$, $y = 2t$, $z = t$; \quad \textbf{5.}~$\textbf{v}(t) = (1,1 - \cos t,\sin t)$,
$\textbf{a}(t) = (0,\sin t,\cos t)$; \quad
\textbf{9.} 
(a)~Line parallel to $\mathbf{c}$; \quad 
(b)~Half-line parallel to $\mathbf{c}$; \quad 
(c)~ Hint:  Think of the functions as position vectors; \quad
\textbf{15.}~Hint: Theorem \ref{thm:vectripleprod}.

\subsection*{Section \ref{sec1dot9} (p. \pageref{sec1dot9})}

\textbf{1.}~$\frac{3\pi \sqrt{5}}{2}$;\quad 
\textbf{3.}~$2 (5^{3/2} - 8)$;\quad 
\textbf{5.}~Replace $t$ by
$\biggl( \biggl( \frac{27s + 16}{2} \biggr)^{2/3} - 4 \biggr)\bigg/ 9$;\quad 
\textbf{6.}~Hint: Use Theorem~\ref{thm:vecdiffprops}(e), Example~\ref{exmp:absvecderiv}, and Theorem~\ref{thm:vectripleprod};\quad 
\textbf{7.}~Hint:
Use Exercise 6.
\textbf{9.}~Hint: Use $\textbf{f}\,'(t) = \norm{\textbf{f}(t)}\textbf{T}$, differentiate that
to get $\textbf{f}\,''(t)$, put those expressions into $\Crossprod{\textbf{f}\,'(t)\,}{\,\textbf{f}\,''(t)}$, then
write $\textbf{T}\,'(t)$ in terms of $\textbf{N}(t)$.;\quad 
\textbf{11.}~$\textbf{T}(t) = \frac{1}{\sqrt{2}}
(-\sin t,\cos t,1)$, $\textbf{N}(t) = (-\cos t,-\sin t,0)$, $\textbf{B}(t) = \frac{1}{\sqrt{2}}(\sin t,-\cos t,1)$,
$\kappa(t) = 1/2$
\section*{Chapter \ref{chapter:mult-var-function}}
\subsection*{Section \ref{sec2dot1} (p. \pageref{sec2dot1})}

\textbf{1.}~domain: $\Real{2}$, range: $\lbrack -1,\infty )$;\quad
\textbf{3.}~domain: $\lbrace (x,y): x^2 + y^2 \ge 4 \rbrace$, range: $\lbrack 0,\infty)$;\quad
\textbf{5.}~domain:
$\Real{3}$, range: $\ival{-1}{1}$;\quad
\textbf{7.}~1;\quad
\textbf{9.}~does not exist;\quad
\textbf{11.}~$2$;\quad
\textbf{13.}~$2$;\quad
\textbf{15.}~$0$;\quad
\textbf{17.}~does not exist.

\subsection*{Section \ref{sec2dot2} (p. \pageref{sec2dot2})}
\textbf{1.}~$\frac{\partial f}{\partial x} = 2x$, $\frac{\partial f}{\partial y} = 2y$;\quad
\textbf{3.}~$\frac{\partial f}{\partial x} = x(x^2 + y + 4)^{-1/2}$,
$\frac{\partial f}{\partial y} = \frac{1}{2}(x^2 + y + 4)^{-1/2}$;\quad
\textbf{5.}~$\frac{\partial f}{\partial x} = ye^{xy} + y$, $\frac{\partial f}{\partial y} = xe^{xy} + x$;\quad
\textbf{7.}~$\frac{\partial f}{\partial x} = 4x^3$, $\frac{\partial f}{\partial y} = 0$; \quad
\textbf{9.}
$\frac{\partial f}{\partial x}=x(x^2 + y^2 )^{-1/2}$, $\frac{\partial f}{\partial y}=y(x^2 + y^2 )^{-1/2}$; \quad\textbf{11.}
$\frac{\partial f}{\partial x} = \frac{2x}{3}(x^2 + y + 4)^{-2/3}$,
$\frac{\partial f}{\partial y} = \frac{1}{3}(x^2 + y + 4)^{-2/3}$;\quad
\textbf{13.}
$\frac{\partial f}{\partial x}=-2xe^{-(x^2 + y^2 )}$, $\frac{\partial f}{\partial y}=-2ye^{-(x^2 + y^2 )}$;\quad
\textbf{15.}~$\frac{\partial f}{\partial x} = y\cos(xy)$, $\frac{\partial f}{\partial y} = x\cos(xy)$;\quad
\textbf{17.}~$\frac{\partial^2 f}{\partial x^2} =2$,
$\frac{\partial^2 f}{\partial y^2} = 2$,
$\frac{\partial^2 f}{\partial x \,\partial y} = 0$;\quad
\textbf{19.}
$\frac{\partial^2 f}{\partial x^2} = (y+4)(x^2 + y+4)^{-3/2}$, 
$\frac{\partial^2 f}{\partial y^2} = -\frac{1}{4}(x^2 + y+4)^{-3/2}$, 
$\frac{\partial^2 f}{\partial x \,\partial y} = -\frac{1}{2}x(x^2 + y+4)^{-3/2}$; \quad\textbf{21.}
$\frac{\partial^2 f}{\partial x^2} = y^2 e^{xy}$,
$\frac{\partial^2 f}{\partial y^2} = x^2 e^{xy}$,
$\frac{\partial^2 f}{\partial x \,\partial y} = (1+xy)e^{xy} + 1$;\quad
\textbf{23.}~$\frac{\partial^2 f}{\partial x^2} =12x^2$,
$\frac{\partial^2 f}{\partial y^2} = 0$,
$\frac{\partial^2 f}{\partial x \,\partial y} = 0$;\quad
\textbf{25.}~$\frac{\partial^2 f}{\partial x^2} =-x^{-2}$,
$\frac{\partial^2 f}{\partial y^2} = -y^{-2}$,
$\frac{\partial^2 f}{\partial x \,\partial y} = 0$

\subsection*{Section \ref{sec2dot3} (p. \pageref{sec2dot3})}

\textbf{1.}~$2x+3y-z-3=0$;\quad
\textbf{3.}~$-2x+y-z-2=0$;\quad
\textbf{5.}~$x+2y=z$;\quad
\textbf{7.}~$\frac{1}{2}(x-1)+\frac{4}{9}(y-2)+\frac{\sqrt{11}}{12}(z-\frac{2\sqrt{11}}{3})=0$;\quad
\textbf{9.}~$3x+4y-5z=0$.

\subsection*{Section \ref{sec2dot4} (p. \pageref{sec2dot4})}

\textbf{1.}~$(2x,2y)$;\quad
\textbf{3.}~$(\frac{x}{\sqrt{x^2 + y^2 + 4}},\frac{y}{\sqrt{x^2 + y^2 + 4}})$;\quad
\textbf{5.}~$(1/x,1/y)$;\quad
\textbf{7.}~$(yz\cos(xyz),xz\cos(xyz),xy\cos(xyz))$; \quad
\textbf{9.}~$(2x,2y,2z)$;\quad
\textbf{11.}~$2\sqrt{2}$;\quad
\textbf{13.}~$\frac{1}{\sqrt{3}}$;\quad
\textbf{15.}~$\sqrt{3}\,\cos(1)$;\quad
\textbf{17.}~increase: $(45,20)$, decrease: $(-45,-20)$

\subsection*{Section \ref{sec2dot5} (p. \pageref{sec2dot5})}

\textbf{1.}~local min. $(1,0)$; saddle pt. $(-1,0)$; \quad\textbf{3.}
local min. $(1,1)$; local max. $(-1,-1)$; saddle pts. $(1,-1),(-1,1)$;\quad
\textbf{5.}~local min. $(1,-1)$, saddle pt. $(0,0)$;\quad
\textbf{7.}~local min. $(0,0)$;\quad
\textbf{9.}~local min. $(-1,1/2)$;\quad
\textbf{11.}
width = height = depth=$10$;\quad
\textbf{13.}~$x=y=4$, $z=2$.

\subsection*{Section \ref{sec2dot6} (p. \pageref{sec2dot6})}

\textbf{2.}~$(\ssub{x}{0},\ssub{y}{0})=(0,0):$ $\rightarrow (0.2858,-0.3998)$;
$(\ssub{x}{0},\ssub{y}{0})=(1,1):$ $\rightarrow (1.03256,-1.94037)$
\subsection*{Section \ref{sec2dot7} (p. \pageref{sec2dot7})}

\textbf{1.}~min. $\left(\frac{-4}{\sqrt{5}},\frac{-2}{\sqrt{5}}\right)$;
max. $\left(\frac{4}{\sqrt{5}},\frac{2}{\sqrt{5}}\right)$
; \quad
\textbf{3.}
min. $\left(\frac{20}{\sqrt{13}},\frac{30}{\sqrt{13}}\right)$;
max. $\left(-\frac{20}{\sqrt{13}},-\frac{30}{\sqrt{13}}\right)$
\textbf{4.}~There is no global maximum, nor global minimum.
\textbf{5.}~$\frac{8abc}{3\sqrt{3}}$
\section*{Chapter \ref{chapter:mult-integrals}}
\subsection*{Section \ref{sec3dot1} (p. \pageref{sec3dot1})}
\textbf{1.}~$1$;\quad
\textbf{3.}~$\frac{7}{12}$;\quad
\textbf{5.}~$\frac{7}{6}$;\quad
\textbf{7.}~$5$;\quad
\textbf{9.}~$\frac{1}{2}$;\quad
\textbf{11.}~$15$.
\subsection*{Section \ref{sec3dot2} (p. \pageref{sec3dot2})}
\textbf{1.}~$1$;\quad
\textbf{3.}~$8\ln 2 - 3$;\quad
\textbf{5.}~$\frac{\pi}{4}$;\quad
\textbf{6.}~$\frac{1}{4}$;\quad
\textbf{7.}~$2$;\quad
\textbf{9.}~$\frac{1}{6}$;\quad
\textbf{10.}~$\frac{6}{5}$.
\subsection*{Section \ref{sec3dot3} (p. \pageref{sec3dot3})}

\textbf{1.}~$\frac{9}{2}$;\quad
\textbf{3.}~$(2\cos(\pi^2) + \pi^4 -2)/4$;\quad
\textbf{5.}~$\frac{1}{6}$;\quad
\textbf{7.}~$6$; \quad
\textbf{10.}~$\frac{1}{3}$
\subsection*{Section \ref{sec3dot4} (p. \pageref{sec3dot4})}
\textbf{1.}~The values should converge to $\approx 1.318$. (Hint: In Java the exponential function $e^x$ can be obtained
with \texttt{Math.exp(x)}. Other languages have
similar functions, otherwise use $e=2.7182818284590455$ in your program.)
\textbf{2.}~$\approx 1.146$;\quad
\textbf{3.}~$\approx 0.705$;\quad
\textbf{4.}~$\approx 0.168$.
\subsection*{Section \ref{sec3dot5} (p. \pageref{sec3dot5})}

\textbf{1.}~$8\pi$;\quad
\textbf{3.}~$\frac{4\pi}{3}(8-3^{3/2})$;\quad
\textbf{7.}~$1-\frac{\sin 2}{2}$;\quad
\textbf{9.}~$2\pi ab$

\subsection*{Section \ref{sec3dot6} (p. \pageref{sec3dot6})}

\textbf{1.}~$(1,8/3)$\quad
\textbf{3.}~$(0,\frac{4a}{3\pi})$\quad
\textbf{5.}~$(0,3\pi/16)$;\quad
\textbf{7.}~$(0,0,5a/12)$;\quad
\textbf{9.}~$(7/12,7/12,7/12)$
\subsection*{Section \ref{sec3dot7} (p. \pageref{sec3dot7})}

\textbf{1.}~$\sqrt{\pi}$;\quad
\textbf{2.}~1;\quad
\textbf{6.}~Both are $\frac{n}{(n+1)^2 (n+2)}$;\quad
\textbf{7.}~$\frac{1}{n}$;\quad

\section*{Chapter \ref{chapter:surface-integrals}}
\subsection*{Section \ref{sec4dot1} (p. \pageref{sec4dot1})}

\textbf{1.}~$1/2$;\quad
\textbf{3.}~$23$;\quad
\textbf{5.}~$24\pi$;\quad
\textbf{7.}~$-2\pi$;\quad
\textbf{9.}~$2\pi$
\textbf{11.}~$0$
\subsection*{Section \ref{sec4dot2} (p. \pageref{sec4dot2})}

\textbf{1.}~$0$;\quad
\textbf{3.}~No;\quad
\textbf{4.}~Yes. $F(x,y)=\frac{x^2}{2}-\frac{y^2}{2}$;\quad
\textbf{5.}~No;\quad
\textbf{9.}~
(b)~No. Hint: Think of how $F$ is defined;\quad
\textbf{10.}~Yes. $F(x,y)=axy+bx+cy+d$
\subsection*{Section \ref{sec4dot3} (p. \pageref{sec4dot3})}

\textbf{1.}~$16/15$;\quad
\textbf{3.}~$-5\pi$;\quad
\textbf{5.}~Yes. $F(x,y)=xy^2 + x^3$;\quad
\textbf{7.}~Yes. $F(x,y)=4x^2 y + 2y^2 + 3x$

\subsection*{Section \ref{sec4dot4} (p. \pageref{sec4dot4})}

\textbf{1.}~$216\pi$;\quad
\textbf{2.}~$3$;\quad
\textbf{3.}~$12\pi/5$;\quad
\textbf{7.}~$15/4$
\subsection*{Section \ref{sec4dot5} (p. \pageref{sec4dot5})}

\textbf{1.}~$2\sqrt{2}\,\pi^2$\quad
\textbf{2.}~$(17\sqrt{17} - 5\sqrt{5})/3$\quad
\textbf{3.}~$2/5$;\quad
\textbf{4.}~$2$;\quad
\textbf{5.}~$2\pi (\pi - 1)$;\quad
\textbf{7.}~$67/15$;\quad
\textbf{9.}~$6$; \quad
\textbf{11.}~Yes;\quad
\textbf{13.}~No;\quad
\textbf{19.}~Hint: Think of how a vector field $\textbf{f}(x,y) = P(x,y)\,\textbf{i} + Q(x,y)\,\textbf{j}$ in
$\Real{2}$ can be extended in a natural way to be a vector field in $\Real{3}$.
\subsection*{Section \ref{sec4dot6} (p. \pageref{sec4dot6})}%???NUMERATION

\textbf{1.}~$0$;\quad
\textbf{3.}~$12\sqrt{x^2 + y^2 + z^2}$;\quad
\textbf{5.}~$6(x+y+z)$;\quad

\subsection*{Section \ref{sec4dot7} (p. \pageref{sec4dot7})}
\textbf{1.}~$12\rho$;\quad
\textbf{2.}~$(4\rho^2 -6)e^{-\rho^2}$;\quad
\textbf{3.}~$-\frac{2z}{r^3}\,\textbf{e}_{r} + \frac{1}{r^2}\,\textbf{e}_{z}$;\quad
\textbf{5.}~$\div\textbf{f} = \frac{2}{\rho} - \frac{\sin\theta}{\sin\phi} + \cot\phi$, 
$\curl\textbf{f}
= \cot\phi\,\cos\theta\,\textbf{e}_{\rho} + 2\textbf{e}_{\theta} -2\cos\theta\,\textbf{e}_{\phi}$
\textbf{6.}~Hint: Start by showing that $\textbf{e}_{r} = \cos\theta\,\textbf{i} + \sin\theta\,\textbf{j}$,
$\textbf{e}_{\theta} = -\sin\theta\,\textbf{i} + \cos\theta\,\textbf{j}$, $\textbf{e}_{z} = \textbf{k}$.
\end{multicols}
